The following result shall be useful later. For $n \in N$
\begin{align}
    \int_{-\infty}^{\infty} \dfrac{x^n e^{\frac{-x^2}{2}}}{\sqrt{2\pi}}dx = 
    \begin{cases}
    0 & n\; is\; odd\\
    (n-1)\times...\times3\times1 & n\; is\; even
    \end{cases}
\end{align}
The proof for the above can be found at the end of the solution.
\begin{align}
    Corr(X,Y) = \cfrac{\sigma_{XY}^2}{\sigma_X\sigma_Y}
    \label{dec2015-108:correlationofxy}
\end{align}
We know $X \sim N(0,1)$. Thus,
\begin{align}
    f_X(x) &= \dfrac{e^{\frac{-x^2}{2}}}{\sqrt{2\pi}}\\
    E(X) &= 0\\
    \sigma_X^2 &= 1
\end{align}
\begin{align}
    \sigma_Y^2 = E(Y^2) - E(Y)^2
    \label{dec2015-108:varianceofy}
\end{align}
\begin{align}
    E(Y) &= \int_{-\infty}^{\infty}E(Y|X=x)f_X(x)dx\\
         &= \int_{-\infty}^{\infty}\dfrac{x^3 e^{\frac{-x^2}{2}}}{\sqrt{2\pi}}dx\\
         &= 0
\end{align}
\begin{align}
    E(Y^2) &= \int_{-\infty}^{\infty}E(Y^2|X=x)f_X(x)dx\\
           &= \int_{-\infty}^{\infty}\dfrac{x^6 e^{\frac{-x^2}{2}}}{\sqrt{2\pi}}dx\\
           &= 15
\end{align}
Substituting in \eqref{dec2015-108:varianceofy}
\begin{align}
    \sigma_Y^2 = 15
\end{align}
\begin{align}
    \sigma_{XY}^2 = E(XY) - E(X)E(Y)
    \label{dec2015-108:covarianceofxy}
\end{align}
\begin{align}
    E(XY) &= \int_{-\infty}^{\infty}E(XY|X=x)f_X(x)dx\\
          &= \int_{-\infty}^{\infty}E(xY|X=x)f_X(x)dx\\
          &= \int_{-\infty}^{\infty}xE(Y|X=x)f_X(x)dx\\
          &= \int_{-\infty}^{\infty}\dfrac{x^4 e^{\frac{-x^2}{2}}}{\sqrt{2\pi}}dx\\
          &= 3
\end{align}
Substituting in \eqref{dec2015-108:covarianceofxy}
\begin{align}
    \sigma_{XY}^2 = 3
\end{align}
Substituting in \eqref{dec2015-108:correlationofxy}
\begin{align}
    Corr(X,Y) = \cfrac{3}{\sqrt{15}} > 0
\end{align}
Since $Corr(X,Y) \ne 0$, X and Y are dependent. Thus option 2 is the only correct option.
\textbf{Proof for the integral:}
If n is odd, $\dfrac{x^n e^{\frac{-x^2}{2}}}{\sqrt{2\pi}}$ is an odd function, thus
\begin{align}
    \int_{-\infty}^{\infty} \dfrac{x^n e^{\frac{-x^2}{2}}}{\sqrt{2\pi}}dx = 0
\end{align}
If n is even, 
\begin{align}
    \int_{-\infty}^{\infty} \dfrac{x^n e^{\frac{-x^2}{2}}}{\sqrt{2\pi}}dx = \int_{-\infty}^{\infty} (x^{n-1}) (\dfrac{x e^{\frac{-x^2}{2}}}{\sqrt{2\pi}})dx
\end{align}
Using integration by parts,
\begin{multline}
    \int_{-\infty}^{\infty} \dfrac{x^n e^{\frac{-x^2}{2}}}{\sqrt{2\pi}}dx = \left(x^{n-1}\int \dfrac{x e^{\frac{-x^2}{2}}}{\sqrt{2\pi}}dx\right)\biggr \vert_{-\infty}^{\infty}\\
       - (n-1)\int_{-\infty}^{\infty}x^{n-2}\left(\int \dfrac{x e^{\frac{-x^2}{2}}}{\sqrt{2\pi}}dx\right) dx
\end{multline}
\begin{align}
    &= \left(x^{n-1}(-\dfrac{e^{\frac{-x^2}{2}}}{\sqrt{2\pi}})\right)\biggr \vert_{-\infty}^{\infty}
           - (n-1)\int_{-\infty}^{\infty}x^{n-2}(-\dfrac{e^{\frac{-x^2}{2}}}{\sqrt{2\pi}}) dx\\
    &= (n-1)\int_{-\infty}^{\infty} \dfrac{x^{n-2} e^{\frac{-x^2}{2}}}{\sqrt{2\pi}}dx\\
    &= (n-1)(n-3)\int_{-\infty}^{\infty} \dfrac{x^{n-4} e^{\frac{-x^2}{2}}}{\sqrt{2\pi}}dx\\
    &= (n-1)\times...\times3\times1\int_{-\infty}^{\infty} \dfrac{x^0 e^{\frac{-x^2}{2}}}{\sqrt{2\pi}}dx\\
    &= (n-1)\times...\times3\times1
\end{align}

Alternative proof for the integral:

If n is odd, $\dfrac{x^n e^{\frac{-x^2}{2}}}{\sqrt{2\pi}}$ is an odd function, thus
\begin{align}
    \int_{-\infty}^{\infty} \dfrac{x^n e^{\frac{-x^2}{2}}}{\sqrt{2\pi}}dx = 0
\end{align}
If n is even, let $n = 2k$. We differentiate the following identity k times w.r.t. $\alpha$.
\begin{align}
    \int_{-\infty}^{\infty}e^{-\alpha x^2}dx = \sqrt{\left( \dfrac{\pi}{\alpha}\right)}
\end{align}
On differentiating k times, we get
\begin{align}
    \int_{-\infty}^{\infty}x^{2k}e^{-\alpha x^2} = \dfrac{1\times3\times...\times(2k-1)}{2^k}  \sqrt{\left(\dfrac{\pi}{\alpha^{2k+1}}\right)}
\end{align}
On substituting $\alpha = \dfrac{1}{2}$, we get
\begin{align}
    \int_{-\infty}^{\infty}x^{n}e^{-\frac{x^2}{2}} = 1\times3\times...\times(n-1) \sqrt{2 \pi}
\end{align}
Thus
\begin{align}
     \int_{-\infty}^{\infty} \dfrac{x^n e^{\frac{-x^2}{2}}}{\sqrt{2\pi}}dx = (n-1)\times...\times3\times1
\end{align}
