Covariance between X and Y is $E\brak{XY}-E\brak{X}E\brak{Y}$\\
\begin{lemma}
\begin{align}
    \int_{-\infty}^{\infty}xe^{-\frac{1}{2y}\brak{x-y}^2}\,dx = \sqrt{2\pi}y^\frac{3}{2}
\end{align}
\end{lemma}
\begin{proof}
\begin{align}
    &\int_{-\infty}^{\infty}xe^{-\frac{1}{2y}\brak{x-y}^2}\,dx\\
  =&\int_{-\infty}^{\infty}\brak{x-y}e^{-\frac{1}{2y}\brak{x-y}^2}\,dx+y\int_{-\infty}^{\infty}e^{-\frac{1}{2y}\brak{x-y}^2}\,dx\\
 =&0+\sqrt{2\pi}y^{\frac{3}{2}}\int_{-\infty}^{\infty}\frac{1}{\sqrt{y}\sqrt{2\pi}}e^{\frac{-1}{2\brak{\sqrt{y}}^2}\brak{x-y}^2}\,dx\\
 =&\sqrt{2\pi}y^\frac{3}{2}\lim_{x_0 \to -\infty}Q\brak{\frac{x_0 - y}{\sqrt{y}}}\\
  =&\sqrt{2\pi}y^\frac{3}{2} \ref{twoD/4/twoD/4/eq:4}
\end{align}
\end{proof}
\begin{lemma}
\begin{align}
   E\brak{XY}=&\frac{1}{3}   
\end{align}
\end{lemma}
\begin{proof}
\begin{align}
    E\brak{XY}=&\int_{y=0}^{1}\int_{x=-\infty}^{\infty}xy f_{XY}(x,y)\,dx\,dy\\
    =&\int_{y=0}^{1}\int_{x=-\infty}^{\infty}xy\frac{1}{\sqrt{2\pi y}}e^{\frac{-1}{2y}(x-y)^2}\,dx \,dy\\
    =&\int_{0}^{1}\frac{y}{\sqrt{2\pi y}}(\int_{-\infty}^{\infty}xe^{-\frac{1}{2y}(x-y)^2}\,dx)\,dy\\
    \text{from \eqref{twoD/4/eq:4}}\\
    =&\int_{0}^{1}y^2 \,dy\\
     E\brak{XY}=&\frac{1}{3} \ref{twoD/4/twoD/4/eq:1}
    \end{align}
\end{proof} 
\begin{lemma}
\begin{align}
     E\brak{Y}=&\frac{1}{2}
\end{align}
\end{lemma}
\begin{proof}
Y has marginal probability (y $\in$ (0,1))
\begin{align}
    f_Y(y)=&\int_{-\infty}^{\infty}f_{XY}(x,y)\,dx =1\\
    \implies E\brak{Y}=&\int_{0}^{1} y f_{Y}(y)\,dy\\
    E\brak{Y}=&\frac{1}{2} \ref{twoD/4/twoD/4/eq:2}
\end{align}
\end{proof}
\begin{lemma}
\begin{align}
  E\brak{X}=&\frac{1}{2}   
\end{align}
\end{lemma}
\begin{proof}
\begin{align}
 E\brak{X}=&\int_{y=0}^{1}\int_{x=-\infty}^{\infty}x f_{XY}(x,y)\,dx\,dy\\
    =&\int_{y=0}^{1}\int_{x=-\infty}^{\infty}x\frac{1}{\sqrt{2\pi y}}e^{\frac{-1}{2y}(x-y)^2}\,dx \,dy\\
     =&\int_{0}^{1}\frac{1}{\sqrt{2\pi y}}(\int_{-\infty}^{\infty}xe^{-\frac{1}{2y}(x-y)^2}\,dx)\,dy\\
     \text{from \eqref{twoD/4/eq:4}}\\
    =&\int_{0}^{1}y\,dy\\
E\brak{X}=&\frac{1}{2} \ref{twoD/4/twoD/4/eq:3}
\end{align}
\end{proof}
From \eqref{twoD/4/eq:1},\eqref{twoD/4/eq:2},\eqref{twoD/4/eq:3}
\begin{align}
Cov(X,Y)=&E\brak{XY}-E\brak{X}E\brak{Y}\\
       =&\frac{1}{3}-\frac{1}{2}\times \frac{1}{2}\\
Cov(X,Y)=&\frac{1}{12}
\end{align}