\begin{lemma}
    Let $Y_i$ be a Poisson random variable with mean $1$ for $i$ $\in$ $\brak{1,n^2}$
Then, 
\begin{align}
    \sum \limits_{i}^{n^2} Y_i = X_n   
\end{align}

\end{lemma}
\begin{lemma}
    \begin{align}
         \lim  \limits_{n\to \infty} \frac{X_n-n^2}{n} = \mathcal{N}\brak{0,1}
         \label{poisson/2/central}
    \end{align}
    \label{poisson/2/central/lemma}
\end{lemma}
\begin{proof}
Using the  central limit theorem,
    \begin{align}
        \lim  \limits_{n \to \infty} \frac{Y_1+Y_2+..+Y_{n^2} - n^2}{n} = \mathcal{N}(0,1)
    \end{align}
yielding \eqref{poisson/2/central}.
\end{proof}
\begin{lemma}
    \begin{align}
    Q\brak{2} = \displaystyle{\frac{1}{\sqrt{2\pi}} \int \limits_2^{\infty} e^{-x^2/2}\,dx}
\end{align}
\label{poisson/2/qfunc/lemma}
\end{lemma}
\begin{lemma}
        \begin{align}
            \pr{X_n>k} 
            \\ =& Q\brak{\frac{k-n^2}{n}}
            \label{poisson/2/eq-cdf}
        \end{align}        
        \label{poisson/2/eq-cdf/lemma}
\end{lemma}
\begin{proof}
    For $X \sim \gauss{0}{1}$, using Lemma     \ref{poisson/2/central/lemma},
    \begin{align}
        \pr{X_n>k} 
            =& \pr{X>\frac{k-n^2}{n}}
    \end{align}
    yielding             \eqref{poisson/2/eq-cdf}.
\end{proof}
\begin{lemma}
\begin{align}
    Q\brak{X}=1-Q\brak{-x}
    \label{poisson/2/eq-Qx}
\end{align}
\label{poisson/2/eq-Qx/lemma}
\end{lemma}

% Here, $\mathcal{N}\brak{0,1}$ is normal distribution with unit mean and variance
% Now 
% \begin{align*}
%     \because \,{\frac{1}{\sqrt{2\pi}} \int \limits_{-x}^{\infty} e^{-x^2/2}\,dx}\,=\,{\frac{1}{\sqrt{2\pi}} \int \limits_{-\infty}^x e^{-x^2/2}\,dx}
%     \\ \text{and} \quad \frac{1}{\sqrt{2\pi}} \int \limits_{-\infty}^{\infty} e^{-x^2/2}\,dx\,=1
% \end{align*}
% Also
% \begin{align}
%     \frac{1}{\sqrt{2\pi}} \int \limits_2^{\infty} e^{-x^2/2}\,dx=& Q\brak{2}
% \end{align}
\begin{enumerate}
%\setlength\itemsep{1em}
\item Using Lemma         \ref{poisson/2/eq-cdf/lemma},
\begin{align}
    \lim \limits_{n \to \infty} \pr{X_n > (n+1)^2} =& \lim \limits_{n \to \infty}Q \brak{\frac{(n+1)^2-n^2}{n}}
    \\=&Q\brak{2}
\end{align}
$\mathbf{\therefore}$ \textbf{Option 1 is correct}
\item Using Lemma         \ref{poisson/2/eq-cdf/lemma},
\begin{align}
\begin{split}
    \lim \limits_{n \to \infty} & \pr{X_n \leqslant (n+1)^2}\\ =&1-\lim \limits_{n \to \infty}  \pr{X_n > (n+1)^2}
\end{split}
    \\=&1- \lim \limits_{n \to \infty}Q \brak{\frac{(n+1)^2-n^2}{n}}
    \\=&1- Q \brak{2}
    \\ \ne &  Q\brak{2}
\end{align}
$\mathbf{\therefore}$, from Lemma \ref{poisson/2/qfunc/lemma} \textbf{Option 2 is incorrect}
\item   Using Lemma         \ref{poisson/2/eq-cdf/lemma} and Lemma \ref{poisson/2/eq-Qx/lemma}
\begin{align}
\begin{split}
    \lim \limits_{n \to \infty} & \pr{X_n < (n-1)^2}\\ =&1-\lim \limits_{n \to \infty}  \pr{X_n \geq (n-1)^2}
\end{split}
    \\=&1-\lim \limits_{n \to \infty}Q \brak{\frac{(n-1)^2-n^2}{n}}
    \\=& 1-Q \brak{-2}
    \\=& Q\brak{2}
\end{align}
$\mathbf{\therefore}$ \textbf{Option 3 is also correct}
\item Using Lemma         \ref{poisson/2/eq-cdf/lemma} and Lemma \ref{poisson/2/eq-Qx/lemma},
\begin{align}
   \begin{split}
    \lim \limits_{n \to \infty} & \pr{X_n < (n-2)^2}\\ =&1-\lim \limits_{n \to \infty}  \pr{X_n \geq (n-2)^2}
\end{split}
    \\=&1-\lim \limits_{n \to \infty}Q \brak{\frac{(n-2)^2-n^2}{n}}
    \\=&1- Q \brak{-4}
    \\=& Q\brak{4} < Q \brak{2}
\end{align}
$\mathbf{\therefore}$ \textbf{Option 4 is incorrect}
\end{enumerate}
