Given PDF of X,
\begin{align}
    f(x)=\alpha(x-\mu)^{\alpha-1}e^{-(x-\mu)^{\alpha}}\label{june2014-71:3}
\end{align}
\textbf{Important property}(using in \eqref{june2014-71:1} as $x>\mu$):
Given $x-y>0$ and $-\infty<y<\infty$, then
\begin{align}
    \lim_{x \to -\infty} x-y=0
\end{align}
CDF of X,
\begin{align}
    F(x)&=\int_{-\infty}^x{f(x)\;dx}\\
    &=\int_{-\infty}^x{\alpha(x-\mu)^{\alpha-1}e^{-(x-\mu)^{\alpha}}dx}\\
    &=\int_{-\infty}^x{e^{-(x-\mu)^{\alpha}}d(x-\mu)^{\alpha}}\\
    &=\sbrak{\frac{e^{-(x-\mu)^{\alpha}}}{-1}}_{-\infty}^x\\
    &=-e^{-(x-\mu)^{\alpha}}-\lim_{x \to -\infty} \frac{e^{-(x-\mu)^{\alpha}}}{-1}\label{june2014-71:1}\\
    &=-e^{-(x-\mu)^{\alpha}}+ {e^{-(0)^{\alpha}}}\\
   F(x) &=1-e^{-(x-\mu)^{\alpha}}\label{june2014-71:2}
\end{align}
Hazard function $\beta(x)$,(using \eqref{june2014-71:3} and \eqref{june2014-71:2})
\begin{align}
    \beta(x)&=\frac{f(x)}{1-F(x)}\\
    &=\frac{\alpha(x-\mu)^{\alpha-1}e^{-(x-\mu)^{\alpha}}}{1-(1-e^{-(x-\mu)^{\alpha}})}\\
    &=\frac{\alpha(x-\mu)^{\alpha-1}e^{-(x-\mu)^{\alpha}}}{e^{-(x-\mu)^{\alpha}}}\\
    \beta(x)&=\alpha(x-\mu)^{\alpha-1}
\end{align}
\begin{enumerate}
    \item $\beta(x)$ is not constant for all $\alpha$
    \item $\beta(x)=\alpha(x-\mu)^{\alpha-1}$ is an increasing function for $\alpha<0 \;or\; \alpha>1$ as given $x-\mu>0$ for all x.
    
    \textbf{Proof: }
    Using first derivative test, A function is increasing iff its first derivative is positive for all x. 
    \begin{align}
        \dfrac{d}{dx} \beta(x)&=  \dfrac{d}{dx} \alpha(x-\mu)^{\alpha-1}\\
        &= \alpha(\alpha-1)(x-\mu)^{\alpha-2}\label{june2014-71:0}
    \end{align}
    For \eqref{june2014-71:0} to be positive, (As given $x-\mu>0$)
    \begin{align}
        \alpha(\alpha-1)(x-\mu)^{\alpha-2}&>0\\
        \alpha(\alpha-1)&>0\\
        \implies \alpha \in \brak{-\infty,0}\cup \brak{1,\infty}
    \end{align}
    $\therefore \beta(x)$ an increasing function for some $\alpha$
    \item $\beta(x)$ is dependent of $\alpha$
    \item when $\alpha=1$,
\begin{align}
    \beta(x)&=\alpha(x-\mu)^{0}=\alpha
\end{align}
Therefore the hazard function is independent of $\mu$ when $\alpha=1$.
\end{enumerate}
\textbf{ANSWER: (2) and (4)}