Given X$_{1}=$0, X$_{2}=$2, n=2 and
\begin{align}
    f_{\theta}(x) =\theta \brak{\dfrac{1}{\sqrt{2\pi}}}e^{-\dfrac{1}{2} x^{2}} + \brak{1-\theta}\brak{\dfrac{1}{2}}e^{-\mid x\mid}
\end{align}
Then log of likelihood function is given by
\begin{align}
l(\theta) &= \sum_{i=1}^{i=n} \log f_{\theta}(x_{i})\\
&= \log f_{\theta}(x_{1}) + \log f_{\theta}(x_{2}) \\
&=\log\brak{\theta\brak{\dfrac{1}{\sqrt{2\pi}}}e^{-\dfrac{1}{2}0^{2}}+\brak{1-\theta}\brak{\dfrac{1}{2}}e^{-\mid 0\mid}} \nonumber\\&\hspace{0.75cm}+\log\brak{\theta\brak{\dfrac{1}{\sqrt{2\pi}}} e^{-\dfrac{1}{2}2^{2}}+\brak{1-\theta}\brak{\dfrac{1}{2}}e^{-\mid 2\mid}}
\end{align}
\begin{align}
&=\log\brak{\theta\brak{\dfrac{1}{\sqrt{2\pi}}}+(1-\theta)\brak{\dfrac{1}{2}}}\nonumber\\&\hspace{0.75cm}+\log\brak{\theta\brak{\dfrac{1}{\sqrt{2\pi}}} e^{-2}+\brak{1-\theta}\brak{\dfrac{1}{2}}e^{-2}}\\
&=2\log\brak{\theta\brak{\dfrac{1}{\sqrt{2\pi}}}+\brak{1-\theta}\brak{\dfrac{1}{2}}} -2
\end{align}
Since likelihood $L(\theta) = e^{l(\theta)}$.\\ \\
Likelihood function $L(\theta)$  at $\theta = 0, \frac{1}{2}, 1$ is given by
\begin{enumerate}
    \item At $\theta=0$ \hspace{0.5cm} $L(\theta=0)=\frac{1}{4}e^{-2}=0.0338$\\
    \item At $\theta=1$ \hspace{0.5cm} $L(\theta=1)=\frac{1}{2\pi}e^{-2}=0.0215$\\
    \item At $\theta=\frac{1}{2}$ \hspace{0.2cm}
    $L(\theta=\frac{1}{2})=\brak{\frac{1}{2\sqrt{2\pi}}+\frac{1}{4}}^{2}e^{-2}=0.0273$
\end{enumerate}
Hence the maximum likelihood estimate of $\theta$ is at $\theta=0$
