Since $X$ and $Y$ are exponential random variables with means'
\begin{align}
    E[X] = 1 \text{ and } E[Y] = \frac{1}{2}
\end{align}
Marginal PDFs of $X$ and $Y$  are given by
\begin{align}
    f_X(x)= e^{-x} , x>0 \\
    f_Y(y) = 2e^{-2y} , y>0
\end{align}
CDFs for $X$ and $Y$ are
\begin{align}
    F_X(b) &= \int_0^b f_X(x)\,d_x\\
           &= \int_0^b  e^{-x}\,d_x\\
           &= 1-e^{-b}
\end{align}
\begin{align}
    F_Y(b) &= \int_0^b f_Y(y)\,d_y\\
           &= \int_0^b 2e^{-2y}\,d_y\\
           &= \left[-e^{-2y}\right]_0^b\\
           &= 1-e^{-2b}
\end{align}
Now,
\begin{align}
    \pr{X>2Y|X>Y} &= \dfrac{\pr{X>2Y\,,\,X>Y} }{\pr{X>Y}}\\
                  &= \dfrac{\pr{X>2Y}}{\pr{X>Y}} \label{dec2017-59:simul1}
\end{align}
\begin{align}
    \pr{X>Y} &= \pr{Y<X}\\
             &= E[F_Y(X)]\\
             &= \int_0^\infty F_Y(X)\,f_X(x)\,d_x\\
             &= \int_0^\infty (1-e^{-2x})\,e^{-x}d_x\\
             &= \left[\frac{e^{-x}}{-1} - \frac{e^{-3x}}{-3}\right]_0^\infty\\
            &=(0+1)+\frac{1}{3}(0-1) \\
             &= \frac{2}{3} \label{dec2017-59:simul2}
\end{align}
\begin{align}
    \pr{X>2Y} &= \pr{Y<\frac{X}{2}}\\
              &= E[F_Y(X/2)]\\
              &=  \int_0^\infty F_Y(X/2)\,f_X(x)\,d_x\\
              &= \int_{0}^{\infty}(1-e^{-x})\,e^{-x}d_x\\
              &= \left[\frac{e^{-x}}{-1} - \frac{e^{-2x}}{-2}\right]_0^\infty\\
              &= (0+1) + \frac{1}{2}(0-1)\\
              &= \frac{1}{2} \label{dec2017-59:simul3}
\end{align}
Putting \eqref{dec2017-59:simul2} and \eqref{dec2017-59:simul3} in \eqref{dec2017-59:simul1}
\begin{align}
    \pr{X>2Y\,|\,X>Y} &= \frac{1/2}{2/3}\\
                  &= \frac{3}{4}
\end{align}
$\therefore$ Option 4 is the correct answer.